changed definition to be more faithful to original formalization

coq/pcc/temp2.v
@@ -1,41 +1,61 @@
 Require Import List.
+Require Import ssreflect.
 
-
-Inductive configuration := a | a' | b | b' | x.
-
-
-Inductive trans : configuration -> configuration -> Prop
-(* every A  is followed by B  (and every B  is preceeded by A)
-   every B' is followed by A' (and every A' is preceeded by B) *)
-
-
+Inductive configuration : Set :=
+  | x : configuration
+  | a : nat -> configuration
+  | a' : nat -> configuration
+  | b : nat -> configuration
+  | b' : nat -> configuration.
 
 Inductive execution : list configuration -> Prop :=
-| exec_nil : execution nil
-| exec_sing : forall c, execution (c :: nil)
-| exec_trans : forall `(trans c c')
-                 `(execution (c' :: e)),
-                 execution (c' :: c :: e).
+  | exec_nil : execution nil
+  | exec_x : forall `(execution e), execution (x :: e)
+  | exec_call : forall `(execution e) (n : nat), execution ((a n):: (b n) :: e)
+  | exec_return : forall `(execution e) (n : nat), execution ((b' n) :: (a' n) :: e).
 
-
-Fixpoint a_confs (e : list configuration) : list configuration :=
+Fixpoint a_confs (e : list configuration) : list nat :=
 match e with
 | nil => nil
-| a  :: e' => a :: a_confs e'
-| a' :: e' => a' :: a_confs e'
-| _  :: e' => a_confs e'
+| a n :: e' => n :: a_confs e'
+| a' n :: e' => n :: a_confs e'
+| _ :: e' => a_confs e'
 end.
 
+Definition test_conf_list := (x :: x :: (a 1) :: (b 1) :: x :: x :: (b' 5) :: (a' 5) :: nil).
 
-Fixpoint b_confs (e : list configuration) : list configuration :=
+Lemma test_exec : execution test_conf_list.
+Proof.
+ rewrite /test_conf_list.
+ apply exec_x.
+ apply exec_x.
+ apply exec_call.
+ apply exec_x.
+ apply exec_x.
+ apply exec_return.
+ apply exec_nil.
+Qed.
+
+Eval compute in a_confs test_conf_list.
+
+Fixpoint b_confs (e : list configuration) : list nat :=
 match e with
 | nil => nil
-| b  :: e' => b :: b_confs e'
-| b' :: e' => b' :: b_confs e'
+| b n  :: e' => n :: b_confs e'
+| b' n :: e' => n :: b_confs e'
 | _  :: e' => b_confs e'
 end.
 
+Eval compute in b_confs test_conf_list.
 
+Lemma test_conf_exists : exists e', (execution e') /\ b_confs test_conf_list = a_confs e'.
+Proof.
+ exists (test_conf_list).
+ split.
+ - by apply test_exec.
+ - done.
+Qed.
+ 
 Lemma exists_exec_with_eq_bs :
   forall `(execution e), exists e', (execution e') /\ b_confs e = a_confs e'.
 Proof.
